CslibTests/HML.lean
@@ -14,15 +14,15 @@ open Cslib Logic Modal HML LTS Model Proposition Satisfies
 open scoped InferenceSystem
 
 example [∀ p μ, Finite ((CCS.lts (defs := defs)).image p μ)] :
-    TheoryEq (Atom := Unit) (ofLTS (CCS.lts (defs := defs)) (fun _ _ => True)) =
-      HomBisimilarity (CCS.lts (defs := defs)) :=
-  theoryEq_eq_bisimilarity ..
+    TheoryEq (HML.Model.toModal
+      ⟨CCS.lts (defs := defs), fun _ (_ : Unit) => True⟩) =
+      HomBisimilarity (CCS.lts (defs := defs)) := theoryEq_eq_bisimilarity ..
 
-example (v : State → Atom → Prop) (htr : lts.Tr s μ s') (hφ : ⇓Modal[ofLTS lts v,s' ⊨ φ]) :
-    ⇓Modal[ofLTS lts v,s ⊨ d⟨μ⟩φ] := by grind only [modal]
+example (m : HML.Model State Label Atom) (htr : m.lts.Tr s μ s')
+    (hφ : ⇓HML[m,s' ⊨ φ]) : ⇓HML[m,s ⊨ d⟨μ⟩φ] := by grind only [modal]
 
-example (v : State → Atom → Prop) (hbox : ⇓Modal[Model.ofLTS lts v,s ⊨ d[μ]φ])
-    (htr : lts.Tr s μ s') : ⇓Modal[ofLTS lts v,s' ⊨ φ] := by grind only [modal]
+example (m : HML.Model State Label Atom) (hbox : ⇓HML[m,s ⊨ d[μ]φ])
+    (htr : m.lts.Tr s μ s') : ⇓HML[m,s' ⊨ φ] := by grind only [modal]
 
 section LogicalEquivalence
 
@@ -36,21 +36,20 @@ principle on the satisfaction relation for the and-connective.
 
 open PFunctor
 
-example {State : Type u} {lts : LTS State Label} {s : State} {μ : Label}
-    {φ₁ φ₂ : HML.Proposition Label Atom} (v : State → Atom → Prop)
-    (h : ⇓Modal[ofLTS lts v,s ⊨ (d⟨μ⟩φ₁) ∧ φ₂]) : ⇓Modal[ofLTS lts v,s ⊨ (¬d[μ]¬φ₁) ∧ φ₂] := by
+example {State : Type u} {m : HML.Model State Label Atom} {s : State} {μ : Label}
+    {φ₁ φ₂ : HML.Proposition Label Atom} (h : ⇓HML[m,s ⊨ (d⟨μ⟩φ₁) ∧ φ₂]) :
+    ⇓HML[m,s ⊨ (¬d[μ]¬φ₁) ∧ φ₂] := by
   let pc : HasContext.Context (HML.Proposition Label Atom) := Context.andL .hole φ₂
   have dual a (φ : HML.Proposition Label Atom) : d⟨a⟩φ ≡[UEquiv (World := State)] ¬d[a]¬φ := by
     grind only [modal, Satisfies.unary_dual]
   have eqv := LawfulCongruence.covariant.elim pc (dual μ φ₁)
   let jc : HasHContext.Context (Judgement State (mkUnary Label) Atom)
-      (HML.Proposition Label Atom) := Judgement.Context.mk (ofLTS lts v) s
+      (HML.Proposition Label Atom) := Judgement.Context.mk m.toModal s
   apply LogicalEquivalence.eqvFillValid eqv jc h
 
-example {State : Type u} {lts : LTS State Label} {s : State} {μ : Label}
-    {φ₁ φ₂ : HML.Proposition Label Atom} (v : State → Atom → Prop)
-    (h : ⇓Modal[ofLTS lts v,s ⊨ (d⟨μ⟩φ₁) ∧ φ₂]) :
-    ⇓Modal[ofLTS lts v,s ⊨ (¬d[μ]¬φ₁) ∧ φ₂] := by grind [modal]
+example {State : Type u} {m : HML.Model State Label Atom} {s : State} {μ : Label}
+    {φ₁ φ₂ : HML.Proposition Label Atom} (h : ⇓HML[m,s ⊨ (d⟨μ⟩φ₁) ∧ φ₂]) :
+    ⇓HML[m,s ⊨ (¬d[μ]¬φ₁) ∧ φ₂] := by grind [modal]
 
 end LogicalEquivalence
 
